Deploying to gh-pages from @ xubaiw/reservoir-index@084ba4d09bae6eaebe8e165f85fbc3ab02d2eb9c 🚀

git/user7230724/lean-projects4/Src/Prover/Set.lean
@@ -18,11 +18,11 @@ infix:50 (priority := high) " ∉ " => not_mem
 def empty (a : Set) : Prop :=
 ¬∃ b, b ∈ a
 
-def nempty (a : Set) : Prop :=
+def nonempty (a : Set) : Prop :=
 ¬empty a
 
-def is_set_succ (n n1 : Set) : Prop :=
-∀ a, a ∈ n1 ↔ a ∈ n ∨ a = n1
+def is_succ (n1 n : Set) : Prop :=
+∀ a, a ∈ n1 ↔ a ∈ n ∨ a = n
 
 def subset (a b : Set) : Prop :=
 ∀ c, c ∈ a → c ∈ b
@@ -32,20 +32,20 @@ infix:50 (priority := high) " ⊆ " => subset
 -- Axioms
 
 axiom ax_ext {a b} : (∀ c, c ∈ a ↔ c ∈ b) → a = b
-axiom ax_reg {a} : nempty a → ∃ b, b ∈ a ∧ ¬∃ c, c ∈ b ∧ c ∈ a
+axiom ax_reg {a} : nonempty a → ∃ b, b ∈ a ∧ ¬∃ c, c ∈ b ∧ c ∈ a
 axiom ax_spec a (P : Set → Prop) : ∃ b, ∀ c, c ∈ b ↔ c ∈ a ∧ P c
 axiom ax_union a : ∃ b, ∀ c d, (d ∈ c ∧ c ∈ a) → d ∈ b
 axiom ax_rep a (P : Set → Set → Prop) : (∀ b, b ∈ a → ∃! c, P b c) →
   ∃ b, ∀ c, c ∈ a → ∃ d, d ∈ b ∧ P c d
-axiom ax_inf : ∃ a b, empty b ∧ b ∈ a ∧ ∀ c, c ∈ a → ∀ d, is_set_succ c d → d ∈ a
+axiom ax_inf : ∃ a b, empty b ∧ b ∈ a ∧ ∀ c, c ∈ a → ∀ d, is_succ d c → d ∈ a
 axiom ax_pow : ∀ a, ∃ b, ∀ c, c ⊆ a → c ∈ b
 
 -- Theorems
 
-theorem not_empty {a} : ¬empty a ↔ nempty a :=
+theorem not_empty {a} : ¬empty a ↔ nonempty a :=
 iff_refl
 
-theorem not_nempty {a} : ¬nempty a ↔ empty a :=
+theorem not_nonempty {a} : ¬nonempty a ↔ empty a :=
 iff_intro not_not_elim not_not_intro
 
 theorem subset_refl {a} : a ⊆ a :=
