git/cruhland/lean4-axiomatic/Lean4Axiomatic/Integer/Impl/Difference/Addition.lean
@@ -1,0 +1,116 @@
+import Lean4Axiomatic.Integer.Impl.Difference.Core
+
+namespace Lean4Axiomatic.Integer.Impl.Difference
+
+/-! ## Addition of formal differences -/
+
+variable {ℕ : Type}
+variable [Natural ℕ]
+
+/--
+Addition of differences.
+
+**Definition intuition**: the sum of two differences should be the net effect
+of applying both of them.
+-/
+def add : Difference ℕ → Difference ℕ → Difference ℕ
+| a——b, c——d => (a + c)——(b + d)
+
+instance addOp : Add (Difference ℕ) := {
+  add := add
+}
+
+/--
+Addition of natural number differences is commutative.
+
+**Proof intuition**: Expand definitions to see that we need to show the
+equivalence of two differences of natural number sums. The left and right
+elements of the differences are directly equivalent via commutativity of
+natural number addition, so convert the differences into ordered pairs and use
+commutativity element-wise.
+-/
+theorem add_comm {a b : Difference ℕ} : a + b ≃ b + a := by
+  revert a; intro (a₁——a₂); revert b; intro (b₁——b₂)
+  show a₁——a₂ + b₁——b₂ ≃ b₁——b₂ + a₁——a₂
+  show (a₁ + b₁)——(a₂ + b₂) ≃ (b₁ + a₁)——(b₂ + a₂)
+  show from_prod (a₁ + b₁, a₂ + b₂) ≃ from_prod (b₁ + a₁, b₂ + a₂)
+  apply AA.subst₁
+  show (a₁ + b₁, a₂ + b₂) ≃ (b₁ + a₁, b₂ + a₂)
+  calc
+    (a₁ + b₁, a₂ + b₂) ≃ _ := AA.substL AA.comm
+    (b₁ + a₁, a₂ + b₂) ≃ _ := AA.substR AA.comm
+    (b₁ + a₁, b₂ + a₂) ≃ _ := Rel.refl
+
+instance add_commutative : AA.Commutative (α := Difference ℕ) (· + ·) := {
+  comm := add_comm
+}
+
+/--
+Adding the same difference on the right of two equivalent differences preserves
+their equivalence.
+
+**Proof intuition**: The property is already intuitively true; imagine
+extending two line segments of the same length by the same amount. So the proof
+just expands all definitions into equalities of sums of natural numbers, and
+performs algebra to obtain the desired result.
+-/
+theorem add_substL {a₁ a₂ b : Difference ℕ} : a₁ ≃ a₂ → a₁ + b ≃ a₂ + b := by
+  revert a₁; intro (n——m); revert a₂; intro (k——j); revert b; intro (p——q)
+  intro (_ : n——m ≃ k——j)
+  have : n + j ≃ k + m := ‹n——m ≃ k——j›
+  show n——m + p——q ≃ k——j + p——q
+  show (n + p)——(m + q) ≃ (k + p)——(j + q)
+  show (n + p) + (j + q) ≃ (k + p) + (m + q)
+  calc
+    (n + p) + (j + q) ≃ _ := AA.expr_xxfxxff_lr_swap_rl
+    (n + j) + (p + q) ≃ _ := AA.substL ‹n + j ≃ k + m›
+    (k + m) + (p + q) ≃ _ := AA.expr_xxfxxff_lr_swap_rl
+    (k + p) + (m + q) ≃ _ := Rel.refl
+
+def add_substitutiveL
+    : AA.SubstitutiveOn Hand.L (α := Difference ℕ) (· + ·) AA.tc (· ≃ ·) (· ≃ ·)
+    := {
+  subst₂ := λ (_ : True) => add_substL
+}
+
+def add_substitutive
+    : AA.Substitutive₂ (α := Difference ℕ) (· + ·) AA.tc (· ≃ ·) (· ≃ ·) := {
+  substitutiveL := add_substitutiveL
+  substitutiveR := AA.substR_from_substL_swap (rS := (· ≃ ·)) add_substitutiveL
+}
+
+/--
+Addition of natural number differences is associative.
+
+**Proof intuition**: Expand definitions to see that we need to show the
+equivalence of two differences of natural number sums. The left and right
+elements of the differences are directly equivalent via associativity of
+natural number addition, so convert the differences into ordered pairs and use
+associativity element-wise.
+-/
+def add_assoc {a b c : Difference ℕ} : (a + b) + c ≃ a + (b + c) := by
+  revert a; intro (n——m); revert b; intro (k——j); revert c; intro (p——q)
+  show (n——m + k——j) + p——q ≃ n——m + (k——j + p——q)
+  show (n + k)——(m + j) + p——q ≃ n——m + (k + p)——(j + q)
+  show ((n + k) + p)——((m + j) + q) ≃ (n + (k + p))——(m + (j + q))
+  show from_prod ((n + k) + p, (m + j) + q)
+     ≃ from_prod (n + (k + p), m + (j + q))
+  apply AA.subst₁
+  show ((n + k) + p, (m + j) + q) ≃ (n + (k + p), m + (j + q))
+  calc
+    ((n + k) + p, (m + j) + q) ≃ _ := AA.substL AA.assoc
+    (n + (k + p), (m + j) + q) ≃ _ := AA.substR AA.assoc
+    (n + (k + p), m + (j + q)) ≃ _ := Rel.refl
+
+def add_associative : AA.Associative (α := Difference ℕ) (· + ·) := {
+  assoc := add_assoc
+}
+
+def addition : Addition.Base (Difference ℕ) := {
+  addOp := addOp
+  add_substitutive := add_substitutive
+  add_commutative := add_commutative
+  add_associative := add_associative
+}
+
+end Lean4Axiomatic.Integer.Impl.Difference
