git/cruhland/lean4-axiomatic/Lean4Axiomatic/Integer/Impl/Difference/Core.lean
@@ -1,0 +1,174 @@
+import Lean4Axiomatic.Integer
+import Lean4Axiomatic.Natural
+
+namespace Lean4Axiomatic.Integer.Impl
+
+/-! ## Implementation of fundamental definitions and properties of integers -/
+
+/-! ### Formal difference representation of integers -/
+
+/--
+The formal (as in "having the form of") difference between two values of the
+same type.
+
+The field names suggest an interpretation for this structure of a starting
+value (`init`) that has a quantity (`take`) removed from it. The structure then
+denotes the value of the result.
+
+Equivalently, this structure can be viewed as measuring the "directed gap"
+between the two values. Specifically, it denotes the value that, when combined
+with `take`, gives the result `init`.
+
+Given a type of natural numbers `ℕ`, integers can be defined as values of
+`Difference ℕ` under an equivalence relation that considers two differences to
+be equal when they denote the same value according to an interpretation above.
+-/
+structure Difference (α : Type) : Type :=
+  init : α
+  take : α
+
+infixl:90 "——" => Difference.mk
+
+namespace Difference
+
+/--
+Create a `Difference` from an ordered pair of values.
+
+**Named parameters**
+- `α`: The type of both elements of the ordered pair.
+-/
+def from_prod {α : Type} : α × α → Difference α
+| (x, y) => x——y
+
+variable {ℕ : Type}
+variable [Natural ℕ]
+
+/-! ### Equivalence -/
+
+/--
+The equivalence relation that separates all `Difference ℕ` values into buckets
+denoting integers.
+
+In other words, given two differences `d₁` and `d₂`, they represent the same
+integer if and only if `eqv d₁ d₂` holds.
+
+**Definition intuition**: Equating two differences means that they represent
+the same quantity after subtraction; i.e., after their `take` values have been
+removed from their `init` values. The subtracted values can be removed from the
+equation without changing its correctness by adding each of them to both sides.
+Doing that produces the expression that is the definition of this relation.
+-/
+def eqv : Difference ℕ → Difference ℕ → Prop
+| a——b, c——d => a + d ≃ c + b
+
+-- This is an instance so the operator can be used in the rest of the file
+instance tildeDash : Operators.TildeDash (Difference ℕ) := {
+  tildeDash := eqv
+}
+
+/--
+The equivalence relation on differences is reflexive.
+
+**Proof intuition**: The underlying equality in the equivalence relation is
+symmetric in terms of the two differences; when both differences are the same,
+the equality is trivial.
+-/
+theorem refl {a : Difference ℕ} : a ≃ a := by
+  revert a; intro (a₁——a₂)
+  show a₁ + a₂ ≃ a₁ + a₂
+  exact Rel.refl
+
+/--
+The equivalence relation on differences is symmetric.
+
+**Proof intuition**: The underlying equality in the equivalence relation is
+already symmetric in terms of the two differences.
+-/
+theorem symm {a b : Difference ℕ} : a ≃ b → b ≃ a := by
+  revert a; intro (a₁——a₂); revert b; intro (b₁——b₂)
+  intro (_ : a₁ + b₂ ≃ b₁ + a₂)
+  show b₁ + a₂ ≃ a₁ + b₂
+  exact Rel.symm ‹a₁ + b₂ ≃ b₁ + a₂›
+
+/--
+The equivalence relation on differences is transitive.
+
+**Proof intuition**: Add the underlying equalities of the two hypotheses; this
+nearly produces the goal equality, but both sides have an extra `b₂ + b₁`. Use
+the cancellation property of natural number addition to remove it.
+
+The bulk of the proof is just the algebra needed to prepare for cancellation.
+-/
+theorem trans {a b c : Difference ℕ} : a ≃ b → b ≃ c → a ≃ c := by
+  revert a; intro (a₁——a₂); revert b; intro (b₁——b₂); revert c; intro (c₁——c₂)
+  intro (_ : a₁ + b₂ ≃ b₁ + a₂) (_ : b₁ + c₂ ≃ c₁ + b₂)
+  show a₁ + c₂ ≃ c₁ + a₂
+  have : (a₁ + c₂) + (b₂ + b₁) ≃ (c₁ + a₂) + (b₂ + b₁) := calc
+    (a₁ + c₂) + (b₂ + b₁) ≃ _ := AA.expr_xxfxxff_lr_swap_rl
+    (a₁ + b₂) + (c₂ + b₁) ≃ _ := AA.substL ‹a₁ + b₂ ≃ b₁ + a₂›
+    (b₁ + a₂) + (c₂ + b₁) ≃ _ := AA.substL AA.comm
+    (a₂ + b₁) + (c₂ + b₁) ≃ _ := AA.substR AA.comm
+    (a₂ + b₁) + (b₁ + c₂) ≃ _ := AA.substR ‹b₁ + c₂ ≃ c₁ + b₂›
+    (a₂ + b₁) + (c₁ + b₂) ≃ _ := AA.comm
+    (c₁ + b₂) + (a₂ + b₁) ≃ _ := AA.expr_xxfxxff_lr_swap_rl
+    (c₁ + a₂) + (b₂ + b₁) ≃ _ := Rel.refl
+  exact AA.cancelR ‹(a₁ + c₂) + (b₂ + b₁) ≃ (c₁ + a₂) + (b₂ + b₁)›
+
+instance eqvOp : Relation.Equivalence.EqvOp (Difference ℕ) := {
+  toTildeDash := tildeDash
+  refl := refl
+  symm := symm
+  trans := trans
+}
+
+/--
+Conversion of ordered pairs into `Difference`s preserves equivalence.
+
+**Proof intuition**: Equivalence of ordered pairs is stricter than equivalence
+of differences. For ordered pairs, both the left and right elements must be
+equivalent; for differences, any values representing the same gap are
+equivalent. Thus one only needs to show that the former is strong enough to
+imply the latter.
+-/
+instance from_prod_substitutive
+    : AA.Substitutive₁ (α := ℕ × ℕ) from_prod (· ≃ ·) (· ≃ ·)
+    := by
+  apply AA.Substitutive₁.mk
+  intro p q; revert p; intro ((n, m)); revert q; intro ((k, j))
+  intro (_ : (n, m) ≃ (k, j))
+  show from_prod (n, m) ≃ from_prod (k, j)
+  show n——m ≃ k——j
+  show n + j ≃ k + m
+  have (And.intro (_ : n ≃ k) (_ : m ≃ j)) :=
+    Relation.Equivalence.Impl.Prod.eqv_defn.mp ‹(n, m) ≃ (k, j)›
+  calc
+    n + j ≃ _ := AA.substL ‹n ≃ k›
+    k + j ≃ _ := AA.substR (Rel.symm ‹m ≃ j›)
+    k + m ≃ _ := Rel.refl
+
+instance equality : Equality (Difference ℕ) := {
+  eqvOp := eqvOp
+}
+
+/-! ### Conversion -/
+
+/--
+Every natural number can be represented as a difference.
+
+Frequently used to convert natural number literals into differences, so it's
+defined as an `abbrev` so the typechecker will always expand it.
+
+**Definition intuition**: Taking nothing away from a natural number preserves
+its value.
+-/
+abbrev from_natural : Coe ℕ (Difference ℕ) := {
+  coe := (·——0)
+}
+
+instance conversion : Conversion ℕ (Difference ℕ) := {
+  from_natural := from_natural
+}
+
+end Difference
+
+end Lean4Axiomatic.Integer.Impl
