git/forked-from-1kasper/lean-vcpu/Machine/Simulator.lean
@@ -1,0 +1,138 @@
+import Machine.Parser
+import Machine.Options
+import Lean.Elab
+
+open Lean Machine.Types
+
+namespace List
+  def forAll {α : Type u} (P : α → Prop) : List α → Prop
+  | []      => True
+  | x :: xs => P x ∧ forAll P xs
+
+  def successively {α : Type u} (R : α → α → Prop) : List α → Prop
+  | []           => True
+  | [x]          => True
+  | x :: y :: ys => R x y ∧ successively R (y :: ys)
+
+  def forLast {α : Type u} (P : α → Prop) : List α → Prop
+  | []      => True
+  | [x]     => P x
+  | x :: xs => forLast P xs
+
+  def forFirst {α : Type u} (P : α → Prop) : List α → Prop
+  | []      => True
+  | x :: xs => P x
+
+  def nonempty {α : Type u} : List α → Prop
+  | []      => False
+  | x :: xs => True
+end List
+
+namespace Machine.Types
+  def machine.next : machine → machine
+  | ⟨stack, regs, flag, progc⟩ => ⟨stack, regs, flag, progc + 1⟩
+
+  def machine.get (m : machine) (r : reg) : Int :=
+  (m.regs.find? r).get!
+end Machine.Types
+
+namespace Machine.Simulator
+  def condjmp (M : machine) (cond : Ordering) (ptr : Nat) : machine :=
+  ⟨M.stack, M.regs, M.flag, if M.flag == cond then ptr else M.progc + 1⟩
+
+  def instr.eval (M : machine) : instr → machine
+  | instr.push z => ⟨M.stack.push z, M.regs, M.flag, M.progc + 1⟩
+  | instr.pushr r => ⟨M.stack.push (M.get r), M.regs, M.flag, M.progc + 1⟩
+  | instr.popr r => ⟨M.stack.pop, M.regs.replace r M.stack.back, M.flag, M.progc + 1⟩
+  | instr.dup => ⟨M.stack.push M.stack.back, M.regs, M.flag, M.progc + 1⟩
+  | instr.add r₁ r₂ r₃ => ⟨M.stack, M.regs.replace r₃ (M.get r₁ + M.get r₂), M.flag, M.progc + 1⟩
+  | instr.neg r₁ r₂ => ⟨M.stack, M.regs.replace r₂ (-M.get r₁), M.flag, M.progc + 1⟩
+  | instr.mul r₁ r₂ r₃ => ⟨M.stack, M.regs.replace r₃ (M.get r₁ * M.get r₂), M.flag, M.progc + 1⟩
+  | instr.cmp r₁ r₂ => ⟨M.stack, M.regs, compare (M.get r₁) (M.get r₂), M.progc + 1⟩
+  | instr.jmp ptr => ⟨M.stack, M.regs, M.flag, ptr⟩
+  | instr.je ptr => condjmp M Ordering.eq ptr
+  | instr.jg ptr => condjmp M Ordering.gt ptr
+  | instr.jl ptr => condjmp M Ordering.lt ptr
+  | instr.dump => M.next
+
+  def instr.effect (M : machine) : instr → IO Unit
+  | instr.dump => do println! "r1 = {M.get reg.r1}, r2 = {M.get reg.r2}, r3 = {M.get reg.r3}, r4 = {M.get reg.r4}"
+  | _          => return ()
+
+  def tick (M : machine) (ρ : tape) : Option machine :=
+  match ρ.get? M.progc with
+  | none   => none
+  | some ε => some (instr.eval M ε)
+
+  def effect (M : machine) (ρ : tape) : IO Unit :=
+  match ρ.get? M.progc with
+  | none   => return ()
+  | some ε => instr.effect M ε
+
+  private def await (M₀ : machine) (ρ : tape) : Nat → IO Unit
+  |   0   => throw (IO.userError "execution depth was reached")
+  | n + 1 => do effect M₀ ρ; match tick M₀ ρ with
+    | none   => return ()
+    | some M => await M ρ n
+
+  private partial def unsafeAwait (M₀ : machine) (ρ : tape) : IO Unit :=
+  do effect M₀ ρ; match tick M₀ ρ with
+  | none   => return ()
+  | some M => unsafeAwait M ρ
+
+  def simulate :=
+  unsafeAwait machine.init
+
+  elab "asm " label:ident xs:mnemonic* " end" : command => do
+    let (ρ, M) ← Machine.Parser.expand xs
+    let xs ← Array.mapM instr.restore ρ
+    Elab.Command.elabDeclaration (← `(def $label : Array instr := #[$xs,*]))
+
+    let opts ← getOptions
+
+    if Machine.Options.debugAsm.get opts then
+      do await M ρ (Machine.Options.executionDepth.get opts)
+    else return ()
+
+  def computes (ρ : tape) (M₁ M₂ : machine) :=
+  tick M₁ ρ = some M₂
+
+  def completed (ρ : tape) (M : machine) :=
+  tick M ρ = none
+
+  def clean (M : machine) :=
+  M = machine.init
+
+  def allowed (ρ : tape) (L : List machine) :=
+  L.successively (computes ρ) ∧ L.forLast (completed ρ)
+
+  def terminator (ρ : tape) (L : List machine) :=
+  L.nonempty ∧ L.forFirst clean ∧ allowed ρ L
+
+  def terminating (ρ : tape) :=
+  ∃ L, terminator ρ L
+
+  asm loop
+    M: jmp M
+  end
+
+  theorem some_inj {α : Type u} {a b : α} (p : some a = some b) : a = b :=
+  by { apply Option.noConfusion p; apply id }
+
+  theorem loop.conservative : ∀ (M₁ M₂ : machine), tick M₁ loop = M₂ → M₁ = M₂ :=
+  λ ⟨stack₁, regs₁, flags₁, progc₁⟩ ⟨stack₂, regs₂, flags₂, progc₂⟩ H => by {
+    induction progc₁; apply some_inj H; cases H
+  }
+
+  theorem loopTerminator : ∀ (L : List machine), terminator loop L → False
+  | [], ⟨p, _⟩ => p
+  | [x], ⟨_, ⟨q, ⟨_, h⟩⟩⟩ => by { rw [q] at h; cases h }
+  | x :: y :: ys, ⟨p, ⟨q, ⟨r, h⟩⟩⟩ => by {
+    apply loopTerminator (y :: ys); apply And.intro;
+    apply True.intro; apply And.intro; rw [←loop.conservative x y r.left];
+    apply q; apply And.intro; apply r.right; apply h
+  }
+
+  theorem nonterminating : ¬terminating loop :=
+  λ | Exists.intro L η => loopTerminator L η
+end Machine.Simulator
